reify/congruence_prover.v
@@ -1,0 +1,238 @@
+Require Import List.
+Require Import MirrorShard.Expr MirrorShard.Env.
+Require Import Prover.
+Require Import types.
+Require Import expr_equality.
+Require Import ExtLib.Tactics.
+Require Import UnionFind.
+Set Implicit Arguments.
+Set Strict Implicit.
+
+
+
+
+(*TODO, this should be a module over a map, so the map can be changed out *)
+Module CONGRUENCE_PROVER (X: UnionFind.MAP with Definition elt := tvar) 
+(Y: UnionFind.UNIONFIND with Definition elt := expr).
+
+Import Y.
+Section CongruenceProver.
+  Variable types : list type.
+  Variable fs : functions types.
+
+  Definition congruence_summary : Type := X.t (Y.t).
+  
+  Definition congruenceLearnOne (hyp : expr) (sum : congruence_summary)  : congruence_summary :=
+   match hyp with
+   | Equal tv a b => 
+     match (X.get tv sum) with
+       | Some uf => X.set tv (union uf a b) sum
+       | None => X.set tv (union empty a b) sum
+     end
+   | _ => sum
+   end.
+
+   Definition congruenceLearn (sum : congruence_summary) (hyps : exprs) : congruence_summary :=
+   fold_right (congruenceLearnOne) sum hyps.
+
+  Definition congruenceSummarize (hyps : exprs) : congruence_summary := 
+   fold_right (congruenceLearnOne) (X.empty t) hyps.
+
+  Definition congruenceProve (sum : congruence_summary)
+    (goal : expr) : bool :=
+    match goal with
+    | Equal t a b =>
+        match (X.get t sum) with
+          | Some uf =>
+            let (arepr, newsum) := find uf a in
+            let (brepr, newsum) := find newsum b in
+            eq_expr arepr brepr
+          | None => false
+        end
+    | _ => false
+end.
+
+  Definition congruenceValid (uvars vars : env types) (sum : congruence_summary) : Prop :=
+   forall tv a b uf, 
+     a <> b ->
+     X.get tv sum = Some uf ->
+     sameclass uf a b -> 
+     Provable fs uvars vars (Equal tv a b).
+
+  Lemma congruenceValid_extensible : forall u g f ue ge,
+    congruenceValid u g f -> congruenceValid (u ++ ue) (g ++ ge) f.
+  Proof.
+    unfold congruenceValid.
+    intros.
+    (specialize (H tv a b uf)).
+    intuition.
+    intuition. destruct H1.
+    eapply Provable_weaken. eauto.
+  Qed.
+
+Lemma Provable_trans :
+forall {types} (fs : functions types) uvars vars t a b c
+(P1 : Provable fs uvars vars (Equal t a b))
+(P2 : Provable fs uvars vars (Equal t b c)),
+Provable fs uvars vars (Equal t a c). 
+intros.
+unfold Provable in *. simpl in *.
+consider (exprD fs0 uvars vars a t0); intros;
+consider (exprD fs0 uvars vars c t0); intros;
+consider (exprD fs0 uvars vars b t0); intros; subst; auto; contradiction.
+Qed.
+
+Lemma Provable_sym :
+forall {types} (fs : functions types) uvars vars t a b 
+(P1 : Provable fs uvars vars (Equal t a b)),
+Provable fs uvars vars (Equal t b a).
+Proof.
+  intros.
+  unfold Provable in *. simpl in *.
+  consider (exprD fs0 uvars vars a t0); intros;
+  consider (exprD fs0 uvars vars b t0); intros; subst; auto; contradiction.
+Qed.
+
+
+Lemma congruenceLearnCorrect : 
+  forall uvars vars hyps sum
+  (All_Prov : AllProvable fs uvars vars hyps)
+  (CV : congruenceValid uvars vars sum),
+    congruenceValid uvars vars (congruenceLearn sum hyps).
+Proof.
+  intros.
+  unfold congruenceValid in *. intros ? ? ? ? ABNe Map.
+  unfold congruenceLearn in *.
+  generalize dependent uf.
+  generalize dependent a.
+  generalize dependent b.
+  induction hyps as [ | hd_hyp tl_hyp]. 
+  + intros. vm_compute in Map. eapply CV; eauto.
+  + intros b a Ne uf SC Lrn.
+    simpl in *. destruct All_Prov as [PHd AP].
+    unfold congruenceLearnOne at 1 in SC. 
+    destruct hd_hyp; 
+      try solve [eapply IHtl_hyp; eauto].
+    consider ( X.get t0 (fold_right congruenceLearnOne sum tl_hyp)).
+    - intros ? TlLrn NewMap.
+      rewrite X.gsspec in NewMap.
+      consider (X.elt_eq tv t0); intros TvEq.
+        * subst. inversion TvEq; subst; clear TvEq.
+          assert (Lrn2 := Lrn).
+          apply sameclass_union_3 in Lrn.
+          destruct Lrn as [ S | [[S1 S2] | [S1 S2]]]; 
+            try solve [eapply IHtl_hyp; eauto].
+          {
+            destruct (expr_eq_dec a hd_hyp1) as [  | ANE]; subst;
+            destruct (expr_eq_dec b hd_hyp2) as [ | BNE]; subst. 
+            * auto.
+            * eapply IHtl_hyp in S2; eauto.
+              eapply Provable_trans. apply PHd. apply Provable_sym. auto.
+            * eapply IHtl_hyp in S1; eauto. eapply Provable_trans; eauto.
+            * eapply IHtl_hyp in S1; eauto. 
+              eapply IHtl_hyp in S2; eauto. eapply Provable_trans; eauto.
+              eapply Provable_trans; eauto.
+              apply Provable_sym; auto.
+          }
+          
+          {
+            destruct (expr_eq_dec a hd_hyp2) as [  | ANE]; subst;
+            destruct (expr_eq_dec b hd_hyp1) as [ | BNE]; subst. 
+            * apply Provable_sym; auto.
+            * eapply IHtl_hyp in S2; eauto.
+              eapply Provable_trans. apply Provable_sym; eauto.
+              apply Provable_sym; auto.
+            * eapply IHtl_hyp in S1; eauto. 
+              eapply Provable_trans; eauto. apply Provable_sym; auto.
+            * eapply IHtl_hyp in S1; eauto. 
+              eapply IHtl_hyp in S2; eauto. eapply Provable_trans; eauto.
+              apply Provable_sym.
+              eapply Provable_trans; eauto.
+          }
+        * eapply IHtl_hyp; eauto.
+    - rewrite X.gsspec in *. consider (X.elt_eq tv t0); subst.
+      * intros. inversion H0; subst; clear H0.
+        apply sameclass_union_3 in Lrn.
+        destruct Lrn as [ S | [[S1 S2] | [S1 S2]]]; 
+          try solve [eapply IHtl_hyp; eauto];
+          try solve [ try apply sameclass_empty in S1; try apply sameclass_empty in S2; try apply sameclass_empty in S; 
+                      try subst; intuition].
+        
+        apply sameclass_empty in S1. apply sameclass_empty in S2.
+        subst. apply Provable_sym. auto.
+      * intros FR FR2. 
+        eapply IHtl_hyp; eauto.
+Qed.
+
+Lemma congruenceSummarizeCorrect : forall uvars vars hyps
+                                          (All_Prov : AllProvable fs uvars vars hyps),
+                                     congruenceValid uvars vars (congruenceSummarize hyps).
+Proof.
+  intros.
+
+apply congruenceLearnCorrect; auto.
+unfold congruenceValid. intros. 
+rewrite X.gempty in H0.
+ congruence.
+Qed.
+      
+Theorem congruenceProverCorrect : ProverCorrect fs congruenceValid congruenceProve.
+Proof.
+unfold ProverCorrect, ProverCorrect'. 
+intros ? ? ? CV ? CP VP.
+destruct goal; try solve [inversion CP].
+destruct (expr_eq_dec goal1 goal2). subst.
+t.
+unfold congruenceValid in CV.
+unfold congruenceProve in CP.
+consider (X.get t0 sum).
+  + intros t1 S CP.
+    consider (find t1 goal1). intros ? ? F1 CP.
+    consider (find t2 goal2). intros ? ? F2 CP.
+    eapply CV; eauto. 
+    unfold sameclass. 
+    assert (fst (find t1 goal1) = e) as F1_. rewrite F1; auto.
+    rewrite find_repr in F1_.
+    assert (repr t2 goal2 = e0) as F2_. rewrite <- find_repr. 
+    rewrite F2. auto.
+    unfold eq_expr in CP.
+    consider (expr_comp e e0); intros CPr; try congruence.
+    apply expr_comp_eq_iff in CPr. subst. 
+    assert (repr t1 goal2 = repr t2 goal2).
+      assert (t2 = snd (find t1 goal1)). rewrite F1. auto.
+      assert (F2_ := F2).
+    rewrite H in F2 at 2. rewrite find_unchanged in F2. 
+    rewrite F2_ in F2. inversion F2; auto. rewrite H in *; auto.
+Qed.
+
+
+  Definition congruenceProver : ProverT :=
+  {| Facts := congruence_summary
+   ; Summarize := congruenceSummarize
+   ; Learn := congruenceLearn
+   ; Prove := congruenceProve
+   |}.
+
+  Definition congruenceProver_correct : ProverT_correct congruenceProver fs.
+  eapply Build_ProverT_correct with (Valid := congruenceValid);
+    eauto using congruenceSummarizeCorrect, congruenceLearnCorrect, congruenceProverCorrect. intros. apply congruenceValid_extensible; auto.
+  Qed.
+
+End CongruenceProver.
+
+Definition CongruenceProver : ProverPackage :=
+{| ProverTypes := nil_Repr EmptySet_type
+ ; ProverFuncs := fun ts => nil_Repr (Default_signature ts)
+ ; Prover_correct := fun ts fs => congruenceProver_correct fs
+|}.
+
+End CONGRUENCE_PROVER.
+
+Module VST_CONGRUENCE_PROVER := CONGRUENCE_PROVER TVAR_MAP EXPR_UF.
+
+
+
+
+    
+
+    
