reify/expr_equality.v
@@ -1,0 +1,262 @@
+Require Import MirrorShard.Expr.
+Import Compare_dec.
+Require Import List.
+Require Import compcert.lib.Coqlib.
+Require Import ExtLib.Tactics.
+Require Import Equalities.
+Require Import UnionFind.
+Require Import compcert.lib.Maps.
+
+
+Fixpoint tvar_comp t1 t2 : Datatypes.comparison :=
+match t1, t2 with
+| tvProp, tvProp => Eq
+| tvType n1, tvType n2 => nat_compare n1 n2
+| tvProp, _ => Lt
+| _, _ => Gt
+end.
+
+Fixpoint expr_comp a b: Datatypes.comparison :=
+match a, b with  
+| Var x, Var y => nat_compare x y
+| Func f1 l1, Func f2 l2 => 
+     let fcomp := nat_compare f1 f2 in
+     match fcomp with 
+       | Datatypes.Eq => 
+         (fix expr_comp' l1 l2 : Datatypes.comparison :=
+            match l1, l2 with
+              | nil, nil => Datatypes.Eq
+              | h::t, nil => Datatypes.Gt
+              | nil, h::t => Datatypes.Lt
+              | h1::t1, h2::t2 =>
+                let r := (expr_comp h1 h2) in
+                match r  with
+                  | Datatypes.Eq => expr_comp' t1 t2
+                  | _ => r
+                end
+            end) l1 l2
+       | _ => fcomp
+     end
+| Equal t1 e1 e2, Equal t2 e3 e4 =>
+  let r := tvar_comp t1 t2 in
+  match r with
+  | Datatypes.Eq => 
+    let c := expr_comp e1 e3 in
+    match c with
+      | Datatypes.Eq => expr_comp e2 e4
+      | _ => c
+    end 
+  | _ => r
+  end
+| UVar x, UVar y => nat_compare x y
+| Not e1, Not e2 => expr_comp e1 e2
+| Var _, _ => Datatypes.Lt
+| _, Var _ => Datatypes.Gt
+| Func _ _, _ => Datatypes.Lt
+| _, Func _ _ => Datatypes.Gt
+| Equal _ _ _, _ => Datatypes.Lt
+| _, Equal _  _ _ => Datatypes.Gt
+| Not _, _ => Datatypes.Lt
+| _, Not _ => Datatypes.Gt
+end.
+
+Definition eq_expr a b : bool :=
+match expr_comp a b with
+| Datatypes.Eq => true
+| _ => false
+end.
+
+Definition lt_prop_expr a b :=
+match expr_comp a b with
+| Datatypes.Lt => True
+| _ => False
+end.
+
+Lemma nat_compare_refl : forall a, nat_compare a a = Datatypes.Eq.
+Proof.
+induction a. auto.
+simpl. apply IHa.
+Qed.
+
+Lemma nat_compare_sym : forall a b, nat_compare a b = Datatypes.Eq -> 
+                                     nat_compare b a = Datatypes.Eq.
+Proof.
+induction a; intros; auto.
+simpl. destruct b; simpl in *; congruence.
+destruct b; simpl in *; try congruence; apply IHa; auto. 
+Qed.
+
+Lemma eq_expr_refl : forall x : expr, eq_expr x x= true.
+intros;
+induction x; auto.
+  + unfold eq_expr. simpl.
+    rewrite nat_compare_refl. auto.
+  + unfold eq_expr. simpl.
+    rewrite nat_compare_refl. auto.
+  + unfold eq_expr. simpl.
+    rewrite nat_compare_refl. 
+      induction l; auto.
+        -  inv H. unfold eq_expr in H2. destruct (expr_comp a a); inv H2.
+           apply IHl.
+           auto.
+  + unfold eq_expr in *. simpl. destruct t. simpl.
+    destruct (expr_comp x1 x1); inv IHx1.
+    auto.
+    simpl. rewrite nat_compare_refl.
+    destruct (expr_comp x1 x1); inv IHx1.
+    auto.
+Qed.
+
+Lemma expr_comp_refl : forall x, expr_comp x x = Eq.
+Proof.
+intros.
+assert (X := eq_expr_refl x). unfold eq_expr in *.
+consider (expr_comp x x). auto.
+Qed.
+
+Lemma expr_comp_eq_iff : forall a b, expr_comp a b = Eq <-> a = b.
+Proof.
+intros.
+split; intros. generalize dependent b.
+ + induction a; intros; simpl in *; auto.
+     - destruct b; inv H.
+       rewrite nat_compare_eq_iff in H1. auto.
+     - consider b; intros; try congruence.
+       rewrite nat_compare_eq_iff in H0. auto.
+     - destruct b; inv H0.
+       pose (expr_comp' := 
+               (fix expr_comp' (l1 l0 : list expr) {struct l1} :
+                 Datatypes.comparison :=
+                 match l1 with
+                 | nil => match l0 with
+                          | nil => Eq
+                          | _ :: _ => Lt
+                          end
+                 | h1 :: t1 =>
+                     match l0 with
+                     | nil => Gt
+                     | h2 :: t2 =>
+                         match expr_comp h1 h2 with
+                         | Eq => expr_comp' t1 t2
+                         | Lt => expr_comp h1 h2
+                         | Gt => expr_comp h1 h2
+                         end
+                     end
+                 end)).
+       fold expr_comp' in H2.
+       consider (nat_compare f f0); intros; try congruence.
+       rewrite nat_compare_eq_iff in H0. subst. f_equal.
+       generalize dependent l0.
+       induction l; intros. 
+         * consider l0; intros; simpl in *; auto; congruence.
+         * simpl in *. inv H. 
+           consider (l0); intros; try congruence.
+           consider (expr_comp a e); intros; try congruence.
+           rewrite (H3 e) by auto.
+           erewrite IHl by eauto. auto.
+     - consider b; try congruence; intros.
+       consider (expr_comp a1 e); try congruence; intros.
+        assert (t = t0). destruct t, t0; inv H1; auto.
+        consider (nat_compare n n0); intros; try congruence.
+        rewrite nat_compare_eq_iff in *; auto. subst. 
+        erewrite IHa1 by eauto. f_equal.
+        consider (tvar_comp t0 t0); intros; try congruence.
+        eauto.
+        consider (tvar_comp t t0); try congruence.
+        consider (tvar_comp t t0); try congruence.   
+     - destruct b; inv H.
+       erewrite IHa; eauto.
+ + subst. assert (x:= eq_expr_refl b). unfold eq_expr in x.
+   destruct (expr_comp b b); inv x; auto.
+Qed.
+
+Lemma expr_eqb_eq : forall x y : expr, eq_expr x y = true <-> x = y.
+  Proof.
+    unfold eqb, eq_expr; intuition;
+    consider (expr_comp x y); intros;
+    try apply expr_comp_eq_iff in H; auto;
+    subst; try apply expr_comp_refl in H0; congruence.
+    Qed.
+      
+
+Lemma expr_eq_dec : forall (x y: expr), {x=y} + {x<>y}.
+Proof.
+intros.
+case_eq (eq_expr x y); intros.
+apply (expr_eqb_eq x y) in H. subst; auto.
+right. intuition. subst. rewrite eq_expr_refl in H. congruence.
+Defined.
+
+Module Type BOOL_EQUALITY_TYPE.
+  Variable t: Type.
+  Variable beq : t -> t -> bool.
+  Parameter beq_true : forall x y, beq x y = true <-> x = y.
+End BOOL_EQUALITY_TYPE.
+
+Module EXPR_EQUALITY <: BOOL_EQUALITY_TYPE.
+  Definition t := expr.
+  Definition beq := eq_expr.
+  Definition beq_true :=expr_eqb_eq.
+End EXPR_EQUALITY.
+
+Module EMAP_BOOL (X : BOOL_EQUALITY_TYPE) <: UnionFind.MAP.
+  Definition elt := X.t.
+  Definition elt_eq : forall (x y : elt), {x = y} + {x <> y}.
+    unfold elt. intros.
+    case_eq (X.beq x y); intros.
+    apply X.beq_true in H. auto.
+    right.
+    intro. apply X.beq_true in H0. congruence.
+  Defined.
+  Definition t (A : Type) : Type :=  (elt -> option A).
+  Definition empty (A : Type) : t A := fun _ => None. 
+  Definition get {A : Type} (e : elt) (m : t A) : option A := m e. 
+  Definition set  {A: Type} (e: elt) (v : A) (m :t A) : t A :=
+                         fun ne => if X.beq ne e then Some v else m ne.
+  Lemma gempty: forall (A: Type) (x: elt), get x (empty A) = None.
+  Proof.
+    intros. unfold empty. unfold get. auto.
+  Qed.
+
+  Lemma gsspec: forall (A: Type) (x y: elt) (v: A) (m: t A),
+    get x (set y v m) = if elt_eq x y then Some v else get x m.
+    Proof.
+      intros. unfold get, set.
+      case_eq (X.beq x y); intros. rewrite X.beq_true in H.
+      subst. destruct (elt_eq y y); intuition.
+      destruct (elt_eq x y); intuition. rewrite <- X.beq_true in e.
+      congruence.
+    Qed.
+      
+End EMAP_BOOL.
+
+Module EXPR_MAP := EMAP_BOOL EXPR_EQUALITY.
+
+Module EXPR_UF := UF EXPR_MAP.
+
+Definition beq_tvar x y :=
+match x, y with
+| tvProp, tvProp => true
+| tvType n1 , tvType n2 => beq_nat n1 n2
+| _, _ => false
+end.
+
+Lemma beq_tvar_true_iff x y:
+beq_tvar x y = true <-> x = y.
+Proof.
+intuition;
+destruct x,y; simpl in *; try congruence.
+apply beq_nat_true in H. subst; auto.
+rewrite beq_nat_true_iff. inversion H. subst. auto.
+Qed.
+
+Module TVAR_EQUALITY <: BOOL_EQUALITY_TYPE.
+  Definition t := tvar.
+  Definition beq := beq_tvar.
+  Definition beq_true := beq_tvar_true_iff.
+End TVAR_EQUALITY.
+
+Module TVAR_MAP := EMAP_BOOL TVAR_EQUALITY.
+
+
+ 
